semantics.v
@@ -1,5 +1,5 @@
-Require Export heap.       
-Require Export Omega.  
+Require Export heap.           
+Require Export Omega.   
 Require Export hetList. 
 Require Export Coq.Program.Equality. 
 
@@ -33,7 +33,7 @@ Theorem decomposeValFalse : forall t E e, value t -> decompose t E e -> False.
 Proof.
   intros t E e v d. inv d; try solve[inv v]. 
 Qed. 
-
+ 
 (*proves that values cannot be decomposed*)
 Ltac decompVal :=
   match goal with
@@ -89,20 +89,23 @@ Fixpoint fill (E:ctxt) (e:term) :=
   end.
 
 (*
-commit H ==> indicates the log is valid and H contains the new writes from the log
+commit H1 H2:
+  -indicates the log is valid 
+  -HI has writes undone in case we later find a violation (invalid heap)
+  -HV keeps values in place but releases locks (valid heap)
 abort e L ==> log was invalid, resume execution at term e with log L
 *)
 Inductive validateRes : Type := 
-|commit : validateRes
-|abort : term -> read_set -> validateRes. 
+|commit : chkpnt -> heap -> heap -> validateRes 
+|abort : chkpnt -> heap -> validateRes. 
 
-Inductive invalidStamp : nat -> lock -> Prop :=
-| StampStale : forall s s', s < s' -> invalidStamp s (Unlocked s')
-| StampLocked : forall s s'' s', invalidStamp s (Locked s' s''). 
+Inductive invalidStamp (tid : nat) (rv : nat) : lock -> Prop :=
+| StampStale : forall s, rv < s -> invalidStamp tid rv (Unlocked s)
+| StampLocked : forall s s', s <> tid -> invalidStamp tid rv (Locked s s'). 
 
-Inductive validStamp : nat -> lock -> Prop :=
-| LockOwned : forall s s', validStamp s (Locked s s')
-| StampFresh : forall s s', s > s' -> validStamp s (Unlocked s').
+Inductive validStamp (tid : nat) (rv : nat) : lock -> Prop :=
+| LockOwned : forall s, validStamp tid rv (Locked tid s)
+| StampFresh : forall s, rv > s -> validStamp tid rv (Unlocked s).
 
 (* Transactional log validation
  * Validate RV L H WV Res
@@ -114,20 +117,44 @@ Inductive validStamp : nat -> lock -> Prop :=
  *    + commit - validation succeeded
  *    + abort e L - abort, picking up with term `e` and log `L`
  *)
-Inductive validate : stamp -> read_set -> heap -> validateRes -> Prop :=
-|validateNil : forall S H, validate S nil H commit
-|validateRead : forall S lock l v E H L,
-                        lookup H l = Some(v, lock) -> validStamp S lock -> 
-                        validate S L H commit ->
-                        validate S ((l, E, v)::L) H commit
-|validateAbortPropogate : forall S L H x L' e, 
-                            validate S L H (abort e L') ->
-                            validate S (x::L) H (abort e L')
-|validateAbortRead : forall S lock H L E l v v',
-              validate S L H commit -> lookup H l = Some(v, lock) ->
-              invalidStamp S lock ->
-              validate S ((l, E, v')::L) H
-                       (abort (fill E(get(loc l))) L). 
+
+Inductive readTail : forall b, log b -> log b -> Prop :=
+|cTail : forall l v E L, readTail false (Chkpnt l E v L) L
+|rTail : forall b l v L, readTail b (Read b l v L) L.  
+
+Inductive validate (tid : nat) (rv wv : nat) (e0 : term) : forall b, log b -> heap -> validateRes -> Prop :=
+|validNil : forall H, validate tid rv wv e0 false NilLog H (commit (e0, NilLog) H H)
+|validChkpnt : forall lock l v E H HI HV L chkpnt,
+                    lookup H l = Some(v, lock) -> validStamp tid rv lock ->
+                    validate tid rv wv e0 false L H (commit chkpnt HV HI) ->
+                    validate tid rv wv e0 false (Chkpnt l E v L) H (commit (fill E (get (loc l)), L) HV HI)
+|invalidChkpnt : forall lock l v E H HI HV L chkpnt,
+                   lookup H l = Some(v, lock) -> invalidStamp tid rv lock ->
+                   validate tid rv wv e0 false L H (commit chkpnt HI HV) ->
+                   validate tid rv wv e0 false (Chkpnt l E v L) H (abort (fill E (get (loc l)), L) HI)
+|validRead : forall b lock l v H HI HV L chkpnt,
+               lookup H l = Some(v, lock) -> validStamp tid rv lock ->
+               validate tid rv wv e0 b L H (commit chkpnt HI HV) ->
+               validate tid rv wv e0 b (Read b l v L) H (commit chkpnt HI HV)
+|invalidRead : forall b lock l v H HI HV L chkpnt,
+                 lookup H l = Some(v, lock) -> invalidStamp tid rv lock ->
+                 validate tid rv wv e0 b L H (commit chkpnt HI HV) ->
+                 validate tid rv wv e0 b (Read b l v L) H (abort chkpnt HI)
+|validWrite : forall l v v' H HI HV b (L : log b) chkpnt oldV,
+                lookup H l = Some(v, Locked tid oldV) ->
+                validate tid rv wv e0 b L H (commit chkpnt HI HV) ->
+                validate tid rv wv e0 true (Write b l v' L) H
+                         (commit chkpnt (update HI l v' (Unlocked oldV))
+                                 (update HV l v (Unlocked wv)))
+|readPropAbort : forall H chkpnt HI b L L',
+                   validate tid rv wv e0 b L' H (abort chkpnt HI) ->
+                   readTail b L L' ->
+                   validate tid rv wv e0 b L H (abort chkpnt HI)
+|writePropAbort : forall H chkpnt HI b l v v' oldV L,
+                    validate tid rv wv e0 b L H (abort chkpnt HI) ->
+                    lookup HI l = Some(v, Locked tid oldV) ->
+                    validate tid rv wv e0 true (Write b l v' L) H
+                             (abort chkpnt (update HI l v' (Unlocked oldV))). 
 
 Fixpoint open (e:term) (k:nat) (e':term) :=
   match e with
@@ -146,57 +173,60 @@ Fixpoint open (e:term) (k:nat) (e':term) :=
       |inatomic e => inatomic (open e k e')
   end. 
 
-Inductive acquireLock : nat -> lock -> lock -> Prop :=
-| acquireLocked : forall S S', acquireLock S (Locked S S') (Locked S S')
-| acquireUnlocked : forall S S', S' < S -> acquireLock S (Unlocked S') (Locked S S'). 
+Inductive acquireLock (l : location) (v : term) : forall b, log b -> nat -> lock -> lock -> log true -> Prop :=
+| acquireLocked : forall S S' L, acquireLock l v true L S (Locked S S') (Locked S S') L    (*already locked it*)
+| acquireUnlocked : forall b L S S',
+                      S' < S ->
+                      acquireLock l v b L S (Unlocked S') (Locked S S') (Write b l v L).    (*newly acquired*)
 
 Inductive trans_step : heap -> thread -> heap -> thread -> Prop :=
 (*read after write*)
-|t_readStep : forall S RS WS E l t tid v e0 lock H, 
+|t_readStep : forall S (L : log false) E l t tid v e0 lock H, 
                 decompose t E (get (loc l)) -> 
-                lookup H l = Some(v, lock) -> validStamp S lock ->
-                trans_step H (tid, Some(S, e0), RS, WS, t) H
-                           (tid, Some(S, e0), (l, E, v)::RS, WS, fill E v)
-|t_writeLocked : forall S RS WS tid E l t v v' e0 H lock lock',
+                lookup H l = Some(v, lock) -> validStamp tid S lock ->
+                trans_step H (txThread false tid S e0 L t) H
+                           (txThread false tid S e0 (Chkpnt l E v L) (fill E v))
+|t_writeLocked : forall b S L tid E l L' t v v' e0 H lock lock',
                    decompose t E (put (loc l) v) ->
-                   lookup H l = Some(v', lock) -> acquireLock tid lock lock' ->
-                   trans_step H (tid, Some(S,e0),RS,WS,t) (update H l v lock')
-                              (tid, Some(S,e0),RS,((l, v')::WS), fill E unit)
-|t_atomicIdemStep : forall E e t tid RS WS H S,
-                     decompose t E (atomic e) -> S <> None ->
-                     trans_step H (tid, S, RS, WS, t) H (tid, S, RS, WS, fill E e)
-|t_betaStep : forall RS WS E e t v tid S H, 
-              decompose t E (app (lambda e) v) -> S <> None ->
-              trans_step H (tid, S, RS, WS, t) H (tid, S, RS, WS, fill E (open e 0 v))
+                   lookup H l = Some(v', lock) -> acquireLock l v' b L tid lock lock' L' ->
+                   trans_step H (txThread b tid S e0 L t) (update H l v lock')
+                              (txThread true tid S e0 L' (fill E unit))
+|t_atomicIdemStep : forall b E e t tid L H S e0,
+                     decompose t E (atomic e) -> 
+                     trans_step H (txThread b tid S e0 L t) H (txThread b tid S e0 L (fill E e))
+|t_betaStep : forall b L E e t v tid S e0 H, 
+              decompose t E (app (lambda e) v) -> 
+              trans_step H (txThread b tid S e0 L t) H (txThread b tid S e0 L (fill E (open e 0 v)))
 .
 
-Inductive replay_step : heap -> thread -> heap -> thread -> Prop := 
-|r_readStepValid : forall S RS WS tid H E l t v e0 lock, 
-                     decompose t E (get (loc l)) -> 
-                     lookup H l = Some(v, lock) -> validStamp S lock ->
-                     replay_step H (tid, Some(S, e0), RS, WS, t) H
-                                 (tid, Some(S, e0), (l, E, v)::RS, WS, fill E v)
-|r_readStepInvalid : forall S RS WS tid E H l t v e0 lock v', 
+Inductive replay_step : heap -> thread -> heap -> thread -> Prop :=
+(*read after write*)
+|r_readStepValid : forall S (L : log false) E l t tid v e0 lock H, 
+                decompose t E (get (loc l)) -> 
+                lookup H l = Some(v, lock) -> validStamp tid S lock ->
+                replay_step H (txThread false tid S e0 L t) H
+                            (txThread false tid S e0 (Chkpnt l E v L) (fill E v))
+|r_readStepInvalid : forall b S L tid E H l t v e0 lock v', 
                        decompose t E (get (loc l)) -> 
-                       lookup H l = Some(v, lock) -> invalidStamp S lock ->
-                       replay_step H (tid, Some(S, e0), RS, WS, t) H
-                                   (tid, Some(S, e0), (l, E, v')::RS, WS, fill E v')
-|r_writeLocked : forall S RS WS E tid l t v v' e0 H lock lock',
+                       lookup H l = Some(v, lock) -> invalidStamp tid S lock ->
+                       replay_step H (txThread b tid S e0 L t) H
+                                   (txThread b tid S e0 (Read b l v' L) (fill E v'))
+|r_writeLocked : forall b S L tid E l t v v' e0 H lock lock' L',
                    decompose t E (put (loc l) v) ->
-                   lookup H l = Some(v', lock) -> acquireLock tid lock lock' ->
-                   replay_step H (tid, Some(S,e0),RS,WS,t) (update H l v lock')
-                               (tid, Some(S,e0),RS,(l,v')::WS, fill E unit)
-|r_writeInvalid : forall S RS WS E tid l t v v' e0 H lock,
+                   lookup H l = Some(v', lock) -> acquireLock l v' b L tid lock lock' L' ->
+                   replay_step H (txThread b tid S e0 L t) (update H l v lock')
+                               (txThread true tid S e0 L' (fill E unit))
+|r_writeInvalid : forall b S L E tid l t v v' e0 H lock,
                     decompose t E (put (loc l) v) ->
-                    lookup H l = Some(v', lock) -> invalidStamp S lock ->
-                    replay_step H (tid, Some(S,e0), RS, WS, t) H
-                                (tid, Some(S,e0), RS, WS, fill E unit)
-|r_atomicIdemStep : forall E e t RS tid WS H S,
-                     decompose t E (atomic e) -> S <> None ->
-                     replay_step H (tid, S, RS, WS, t) H (tid, S, RS, WS, fill E e)
-|r_betaStep : forall RS WS H tid E e t v S, 
-              decompose t E (app (lambda e) v) -> S <> None ->
-              replay_step H (tid, S, RS, WS, t) H (tid, S, RS, WS, fill E (open e 0 v))
+                    lookup H l = Some(v', lock) -> invalidStamp tid S lock ->
+                    replay_step H (txThread b tid S e0 L t) H
+                                (txThread b tid S e0 L (fill E unit))
+|r_atomicIdemStep : forall b E e t tid L H S e0,
+                     decompose t E (atomic e) -> 
+                     replay_step H (txThread b tid S e0 L t) H (txThread b tid S e0 L (fill E e))
+|r_betaStep : forall b L E e t v tid S e0 H, 
+              decompose t E (app (lambda e) v) -> 
+              replay_step H (txThread b tid S e0 L t) H (txThread b tid S e0 L (fill E (open e 0 v)))
 . 
 
 (*reflexive transitive closure of replay_step*)
@@ -213,30 +243,6 @@ Inductive rewind : heap -> thread -> heap -> thread -> Prop :=
                 rewind H t H' t' -> replay_step H' t' H'' t'' -> 
                 rewind H t H'' t''. 
 
-
-(*
- * writeback WS H H'
- * WS - write set
- * H - initial heap
- * WV - write version
- * H' - Updated heap with WS's effects and locks released
- *)
-Inductive writeback (wv : nat) : write_set -> heap -> heap -> Prop :=
-|WBNil : forall H, writeback wv nil H H
-|WBCons : forall v' l v WS H H'' S S',
-            lookup H l = Some(v, Locked S S') ->
-            writeback wv WS (update H l v (Unlocked wv)) H'' ->
-            writeback wv ((l, v')::WS) H H''
-. 
-
-(*S is the thread ID of the releasing thread*)
-Inductive releaseLocks (S : nat) : write_set -> heap -> heap -> Prop :=
-|releaseEmpty : forall H, releaseLocks S [] H H
-|releaseCons : forall l v H H' S' v' WS,
-                 lookup H l = Some(v, Locked S S') ->
-                 releaseLocks S WS (update H l v' (Unlocked S')) H' ->
-                 releaseLocks S ((l, v')::WS) H H'. 
-
 Definition step_sig := nat -> heap -> pool -> nat -> heap -> pool -> Prop. 
 
 (*common steps (single step)*)
@@ -252,46 +258,43 @@ Inductive c_step (st : step_sig) : step_sig :=
           c_step st C H T2 C' H' T2' -> c_step st C H (Par T1 T2) C' H' (Par T1 T2')
 |c_forkStep : forall C H E e tid t, 
               decompose t E (fork e) ->
-              c_step st C H (Single(tid, None, nil, nil, t)) C H 
-                   (Par (Single(tid, None, nil, nil, fill E unit)) (Single(S tid, None, nil, nil, e)))
+              c_step st C H (Single(noTXThread tid t)) C H 
+                   (Par (Single(noTXThread tid (fill E unit))) (Single(noTXThread (S tid) e)))
 |c_allocStep : forall C H v E t l tid, 
                lookup H l = None -> decompose t E (alloc v) ->
-               c_step st C H (Single(tid, None, nil, nil, t)) (plus 1 C) ((l, v, Unlocked 0)::H)
-                    (Single(tid, None, nil, nil, fill E (loc l)))
-|c_commitStep : forall C H S RS WS v t tid E H' e0, 
-                  validate S RS H commit -> decompose t E (inatomic v) ->
-                  writeback C WS H H' -> 
-                  c_step st C H (Single(tid, Some(S, e0), RS, WS, t)) (plus 1 C)
-                         H' (Single(tid, None, nil, nil, fill E v))
+               c_step st C H (Single(noTXThread tid t)) C ((l, v, Unlocked 0)::H)
+                    (Single(noTXThread tid (fill E (loc l))))
+|c_commitStep : forall b C H HI HV chkpnt S L v t tid E e0, 
+                  validate tid S C e0 b L H (commit chkpnt HI HV) -> decompose t E (inatomic v) ->
+                  c_step st C H (Single(txThread b tid S e0 L t)) (plus 1 C)
+                         HV (Single(noTXThread tid (fill E v)))
 |c_atomicStep : forall C H E e t tid, 
                 decompose t E (atomic e) ->
-                c_step st C H (Single(tid, None, nil, nil, t)) (plus 1 C) H 
-                       (Single(tid, Some(C, fill E(inatomic e)),[],[],fill E (inatomic e)))
+                c_step st C H (Single(noTXThread tid t)) (S C) H 
+                       (Single(txThread false tid C (fill E(inatomic e)) NilLog (fill E (inatomic e))))
 |c_betaStep : forall C H E e t v tid, 
               decompose t E (app (lambda e) v) -> 
-              c_step st C H (Single(tid, None, nil, nil, t)) C H
-                     (Single(tid, None, nil, nil, fill E (open e 0 v)))
-|c_tsExtend : forall C H t S e0 RS WS tid,
-                validate S RS H commit ->
-                c_step st C H (Single(tid, Some(S, e0), RS, WS, t)) (plus 1 C) H
-                       (Single(tid, Some(C, e0), RS, WS, t))
+              c_step st C H (Single(noTXThread tid t)) C H
+                     (Single(noTXThread tid (fill E (open e 0 v))))
+|c_tsExtend : forall b C H t S L e0 tid HI HV chkpnt,
+                validate tid S C e0 b L H (commit chkpnt HI HV) ->
+                c_step st C H (Single(txThread b tid S e0 L t)) (plus 1 C) H
+                       (Single(txThread b tid C e0 L t))
 .
 
 Inductive p_step_ : nat -> heap -> pool -> nat -> heap -> pool -> Prop :=
-|p_abortStep : forall RS WS S H H' tid RS' C e e0 e', 
-                 validate S RS H (abort e' RS') ->
-                 releaseLocks tid WS H H' -> 
-                 p_step_ C H (Single(tid, Some(S, e0), RS, WS, e))
-                        (plus 1 C) H' (Single(tid, Some(C, e0), RS', nil, e'))
+|p_abortStep : forall b L L' S H H' tid C e e0 e', 
+                 validate tid S C e0 b L H (abort (e', L') H') ->
+                 p_step_ C H (Single(txThread b tid S e0 L e))
+                        (plus 1 C) H' (Single(txThread false tid C e0 L' e'))
 .
 
 (*full abort STM semantics (single step)*)
 Inductive f_step_ : nat -> heap -> pool -> nat -> heap -> pool -> Prop :=
-|f_abortStep : forall RS WS RS' S H tid H' C e e0 e', 
-                 validate S RS H (abort e' RS') ->
-                 releaseLocks tid WS H H' -> 
-                 f_step_ C H (Single(tid, Some(S, e0), RS, WS, e)) (plus 1 C) H'
-                         (Single(tid, Some(C, e0), nil, nil, e0))
+|f_abortStep : forall b L L' S H H' tid C e e0 e', 
+                 validate tid S C e0 b L H (abort (e', L') H') ->
+                 f_step_ C H (Single(txThread b tid S e0 L e))
+                        (plus 1 C) H' (Single(txThread false tid C e0 NilLog e0))
 . 
 
 Definition p_step := c_step p_step_.
@@ -321,12 +324,23 @@ Definition postfix {A:Type} (L1 L2 : list A) := exists diff, L2 = diff ++ L1.
 **a stamp number less than the global clock.  The stamp number 
 **constraint probably doesn't belong here, but its handy to have*)
 
+Inductive releaseLocks (tid : nat) : forall b, log b -> heap -> heap -> Prop :=
+|releaseNil : forall H, releaseLocks tid false NilLog H H
+|releaseWrite : forall b l v v' oldV L H H',
+                  releaseLocks tid b L H H' ->
+                  lookup H l = Some(v, Locked tid oldV) ->
+                  releaseLocks tid true (Write b l v' L) H (update H' l v' (Unlocked oldV))
+|releaseRead : forall b L L' H H',
+                 releaseLocks tid b L' H H' ->
+                 readTail b L L' ->
+                 releaseLocks tid b L H H'. 
+
 Inductive poolRewind (C : nat) (H : heap) : pool -> Prop :=
-|rewindSingleNoTX : forall tid e, poolRewind C H (Single(tid, None,nil,nil,e))
-|rewindSingleInTX : forall tid S e0 RS WS e H',
-                      releaseLocks tid WS H H' ->
-                      rewind H' (tid, Some(S,e0),nil,nil,e0) H (tid, Some(S,e0),RS,WS,e) ->
-                      S < C -> poolRewind C H (Single(tid, Some(S,e0),RS,WS,e))
+|rewindSingleNoTX : forall tid e, poolRewind C H (Single(noTXThread tid e))
+|rewindSingleInTX : forall b tid S e0 L e H',
+                      releaseLocks tid b L H H' ->
+                      rewind H' (txThread false tid S e0 NilLog e0) H (txThread b tid S e0 L e) ->
+                      S < C -> poolRewind C H (Single(txThread b tid S e0 L e)) 
 |rewindPar : forall T1 T2, poolRewind C H T1 -> poolRewind C H T2 -> poolRewind C H (Par T1 T2). 
 
  
@@ -351,22 +365,34 @@ Proof.
 Qed. 
 
 (*validation is idempotent*)
-Theorem validateValidate : forall S L H L' e,  
-                             validate S L H (abort e L') ->
-                             validate S L' H commit. 
+(*
+Theorem validateValidate : forall b rv wv e0 tid L H L' e H',
+                             validate tid rv wv e0 b L H (abort (e, L') H') ->
+                             exists chkpnt HI HV, validate tid rv wv e0 false L' H (commit chkpnt HI HV). 
 Proof.
-  intros S L H L' e HYP. dependent induction HYP; eauto. 
-Qed. 
+  intros b rv wv e0 tid L H L' e H' HYP. remember (abort (e, L') H'). 
+  induction HYP.
+  {inv Heqv. }
+  {inv Heqv. }
+  {inv Heqv. exists chkpnt. exists H'. exists HV. assumption. }
+  {inv Heqv. }
+  {inv Heqv. admit. }
+  {inv Heqv. }
+  {inv Heqv. inv H0. 
+Qed.
+*)
 
 (*the log returned in an abort is a postfix of the initial log*)
-Theorem abortLogPostfix : forall S L H L' e, 
-                            validate S L H (abort e L') ->
+(*
+Theorem abortLogPostfix : forall b tid rv wv e e0 tid L H  H',
+                            validate tid rv wv e0 b L H (abort (e, L') H') ->
                             postfix L' L. 
 Proof.
-  intros S L H L' e HYP. remember (abort e L'). induction HYP; try solveByInv. 
+  intros tid S L H L' e HYP. remember (abort e L'). induction HYP; try solveByInv. 
   {apply IHHYP in Heqv. unfold postfix in *. invertHyp.  exists (x::x0). auto. }
   {inv Heqv. unfold postfix. exists [(l, E, v')]. auto. }
 Qed.
+ *)
 
 (*filling an evaluation context with the result of a decomposition
 **yields the initial term that was decomposed *)
