heap.v
@@ -37,5 +37,45 @@ Proof.
   }
 Qed.
 
+Theorem lookupUpdate : forall H l v lock v' lock',
+                         lookup H l = Some(v', lock') -> 
+                         lookup (update H l v lock) l = Some(v, lock). 
+Proof.
+  induction H; intros.
+  {simpl in *. inv H. }
+  {simpl in *. destruct a. destruct p. destruct (eq_nat_dec l l1).
+   {inv H0. simpl. destruct (eq_nat_dec l1 l1); auto. exfalso.
+    apply n. auto. }
+   {simpl in *. destruct (eq_nat_dec l l1).
+    {subst. exfalso. apply n; auto. }
+    {eapply IHlist. eauto. }
+   }
+  }
+Qed.
+
+Theorem updateUpdate : forall H l v v' lock lock',
+                         update (update H l v lock) l v' lock' = update H l v' lock'.
+Proof.
+  induction H; intros; auto.
+  simpl in *. destruct a. destruct p. destruct (eq_nat_dec l n).
+  {simpl. subst. destruct (eq_nat_dec n n); auto. exfalso. apply n0; auto. }
+  {simpl. destruct (eq_nat_dec l n).
+   {contradiction. }
+   {rewrite IHlist. auto. }
+  }
+Qed.
+
+Theorem updateIdempotent : forall H l v lock,
+                             lookup H l  = Some(v, lock) ->
+                             update H l v lock = H.
+Proof.
+  induction H; intros; auto.
+  simpl in *. destruct a. destruct p. destruct (eq_nat_dec l l1).
+  {subst. inv H0. auto. }
+  {rewrite IHlist. auto. assumption. }
+Qed. 
 
 
+
+
+  
